CoqOfRust/move_sui/proofs/move_binary_format/file_format.v
@@ -1,0 +1,11 @@
+Require Import CoqOfRust.CoqOfRust.
+Require Import CoqOfRust.simulations.M.
+
+Require Import move_sui.simulations.move_binary_format.file_format.
+
+Module SignatureToken.
+  Lemma t_beq_is_valid (x y : SignatureToken.t) :
+    SignatureToken.t_beq x y = true <-> x = y.
+  Proof.
+  Admitted.
+End SignatureToken.
