CoqOfRust/move_sui/proofs/move_bytecode_verifier/type_safety.v
@@ -1,11 +1,12 @@
 Require Import CoqOfRust.CoqOfRust.
 Require Import CoqOfRust.simulations.M.
-Require Import CoqOfRust.move_sui.proofs.move_abstract_stack.lib.
-Require Import CoqOfRust.move_sui.simulations.move_abstract_stack.lib.
-Require Import CoqOfRust.move_sui.simulations.move_binary_format.file_format.
-Require Import CoqOfRust.move_sui.simulations.move_bytecode_verifier.type_safety.
-Require Import CoqOfRust.move_sui.simulations.move_vm_runtime.interpreter.
-Require Import CoqOfRust.move_sui.simulations.move_vm_types.values.values_impl.
+Require Import move_sui.proofs.move_abstract_stack.lib.
+Require Import move_sui.proofs.move_binary_format.file_format.
+Require Import move_sui.simulations.move_abstract_stack.lib.
+Require Import move_sui.simulations.move_binary_format.file_format.
+Require Import move_sui.simulations.move_bytecode_verifier.type_safety.
+Require Import move_sui.simulations.move_vm_runtime.interpreter.
+Require Import move_sui.simulations.move_vm_types.values.values_impl.
 
 Import simulations.M.Notations.
 
@@ -13,6 +14,13 @@ Module IsValueOfType.
   Definition t (value : Value.t) (typ : SignatureToken.t) : Prop :=
     match value, typ with
     | ValueImpl.U8 _, SignatureToken.U8 => True
+    | ValueImpl.U16 _, SignatureToken.U16 => True
+    | ValueImpl.U32 _, SignatureToken.U32 => True
+    | ValueImpl.U64 _, SignatureToken.U64 => True
+    | ValueImpl.U128 _, SignatureToken.U128 => True
+    | ValueImpl.U256 _, SignatureToken.U256 => True
+    | ValueImpl.Bool _, SignatureToken.Bool => True
+    | ValueImpl.Address _, SignatureToken.Address => True
     (* TODO: other cases *)
     | _, _ => False
     end.
@@ -20,7 +28,10 @@ End IsValueOfType.
 
 Module IsStackValueOfType.
   Definition t (stack : Stack.t) (abstract_stack : AbstractStack.t SignatureToken.t) : Prop :=
-    List.Forall2 IsValueOfType.t stack.(Stack.value) (AbstractStack.flatten abstract_stack).
+    List.Forall2
+      IsValueOfType.t
+      stack.(Stack.value)
+      (AbstractStack.flatten abstract_stack).
 End IsStackValueOfType.
 
 (** Here we show that all the stack operations on values follow the stack operations on types *)
@@ -32,7 +43,8 @@ Module IsInterpreterContextOfType.
   (** For now we do not use the [locals] but they should be eventually *)
   Definition t
       (locals : Locals.t) (interpreter : Interpreter.t)
-      (type_safety_checker : TypeSafetyChecker.t) : Prop :=
+      (type_safety_checker : TypeSafetyChecker.t) :
+      Prop :=
     IsStackValueOfType.t
       interpreter.(Interpreter.operand_stack)
       type_safety_checker.(TypeSafetyChecker.stack).
@@ -43,6 +55,22 @@ Ltac guard_instruction expected_instruction :=
   match goal with
   | _ : _ = expected_instruction |- _ => idtac
   end.
+
+Ltac unfold_state_monad :=
+  unfold StatePanicResult.bind, StatePanic.bind, StatePanic.bind,
+    "return!toS!", "liftS!", "readS!";
+  cbn.
+
+Ltac destruct_push :=
+  unfold TypeSafetyChecker.Impl_TypeSafetyChecker.push;
+  with_strategy opaque [AbstractStack.push] unfold_state_monad;
+  match goal with
+  | |- context[AbstractStack.push ?item ?stack] =>
+    pose proof (
+      AbstractStack.flatten_push item stack
+    ) as H_push
+  end;
+  destruct AbstractStack.push as [[[[]|] ?stack_ty]|]; cbn; [|exact I | exact I].
 
 Lemma progress
     (ty_args : list _Type.t) (function : loader.Function.t) (resolver : loader.Resolver.t)
@@ -55,19 +83,154 @@ Lemma progress
     execute_instruction ty_args function resolver instruction (pc, locals, interpreter)
   with
   | Panic.Value (Result.Ok _, type_safety_checker'),
-      Panic.Value (Result.Ok _, (_, locals', interpreter')) =>
+    Panic.Value (Result.Ok _, (_, locals', interpreter')) =>
     IsInterpreterContextOfType.t locals' interpreter' type_safety_checker'
   | _, _ => True
   end.
 Proof.
-  destruct instruction eqn:H_instruction_eq; cbn.
+  destruct instruction eqn:H_instruction_eq; cbn;
+    unfold IsInterpreterContextOfType.t, IsStackValueOfType.t in H_interpreter.
   { guard_instruction Bytecode.Pop.
+    unfold_state_monad.
+    pose proof (AbstractStack.flatten_pop type_safety_checker.(TypeSafetyChecker.stack)) as H_pop.
+    destruct AbstractStack.pop as [[operand stack'] |]; cbn; [|exact I].
+    destruct operand as [operand|]; cbn; [|exact I].
+    rewrite H_pop in H_interpreter.
     admit.
   }
   { guard_instruction Bytecode.Ret.
     admit.
   }
   { guard_instruction (Bytecode.BrTrue z).
+    unfold_state_monad.
+    pose proof (AbstractStack.flatten_pop type_safety_checker.(TypeSafetyChecker.stack)) as H_pop.
+    destruct AbstractStack.pop as [[operand_ty stack'] |]; cbn; [|exact I].
+    destruct operand_ty as [operand_ty|]; cbn; [|exact I].
+    rewrite H_pop in H_interpreter; clear H_pop.
+    pose proof SignatureToken.t_beq_is_valid operand_ty SignatureToken.Bool as H_beq.
+    destruct SignatureToken.t_beq; cbn; [|exact I].
+    replace operand_ty with SignatureToken.Bool in H_interpreter by sfirstorder; clear H_beq.
+    unfold Stack.Impl_Stack.pop_as, Stack.Impl_Stack.pop; cbn.
+    unfold_state_monad.
+    destruct interpreter, operand_stack; cbn in *.
+    inversion_clear H_interpreter as [|operand ? stack ? H_operand_bool H_stack]; cbn.
+    assert (exists b, operand = ValueImpl.Bool b) as [b H_operand_eq]. {
+      destruct operand; cbn; try contradiction; sfirstorder.
+    }
+    rewrite H_operand_eq; clear H_operand_eq; cbn.
+    apply H_stack.
+  }
+  { guard_instruction (Bytecode.BrFalse z).
+    unfold_state_monad.
+    pose proof (AbstractStack.flatten_pop type_safety_checker.(TypeSafetyChecker.stack)) as H_pop.
+    destruct AbstractStack.pop as [[operand_ty stack'] |]; cbn; [|exact I].
+    destruct operand_ty as [operand_ty|]; cbn; [|exact I].
+    rewrite H_pop in H_interpreter; clear H_pop.
+    pose proof SignatureToken.t_beq_is_valid operand_ty SignatureToken.Bool as H_beq.
+    destruct SignatureToken.t_beq; cbn; [|exact I].
+    replace operand_ty with SignatureToken.Bool in H_interpreter by sfirstorder; clear H_beq.
+    unfold Stack.Impl_Stack.pop_as, Stack.Impl_Stack.pop; cbn.
+    unfold_state_monad.
+    destruct interpreter, operand_stack; cbn in *.
+    inversion_clear H_interpreter as [|operand ? stack ? H_operand_bool H_stack]; cbn.
+    assert (exists b, operand = ValueImpl.Bool b) as [b H_operand_eq]. {
+      destruct operand; cbn; try contradiction; sfirstorder.
+    }
+    rewrite H_operand_eq; clear H_operand_eq; cbn.
+    apply H_stack.
+  }
+  { guard_instruction (Bytecode.Branch z).
+    apply H_interpreter.
+  }
+  { guard_instruction (Bytecode.LdU8 z).
+    destruct_push.
+    lib.step; cbn; [|exact I].
+    unfold IsInterpreterContextOfType.t; cbn.
+    unfold IsStackValueOfType.t; cbn.
+    rewrite H_push.
+    hauto l: on.
+  }
+  { guard_instruction (Bytecode.LdU64 z).
+    destruct_push.
+    lib.step; cbn; [|exact I].
+    unfold IsInterpreterContextOfType.t; cbn.
+    unfold IsStackValueOfType.t; cbn.
+    rewrite H_push.
+    hauto l: on.
+  }
+  { guard_instruction (Bytecode.LdU128 z).
+    destruct_push.
+    lib.step; cbn; [|exact I].
+    unfold IsInterpreterContextOfType.t; cbn.
+    unfold IsStackValueOfType.t; cbn.
+    rewrite H_push.
+    hauto l: on.
+  }
+  { guard_instruction Bytecode.CastU8.
+    unfold_state_monad.
+    pose proof (
+      AbstractStack.flatten_pop type_safety_checker.(TypeSafetyChecker.stack)
+    ) as H_pop.
+    destruct AbstractStack.pop as [[[operand_ty |] stack_ty] |]; cbn; [|exact I | exact I].
+    lib.step; cbn; [exact I|].
+    destruct_push.
+    admit.
+  }
+  { guard_instruction Bytecode.CastU64.
+    admit.
+  }
+  { guard_instruction Bytecode.CastU128.
+    admit.
+  }
+  { guard_instruction (Bytecode.LdConst t).
+    admit.
+  }
+  { guard_instruction Bytecode.LdTrue.
+    admit.
+  }
+  { guard_instruction Bytecode.LdFalse.
+    admit.
+  }
+  { guard_instruction (Bytecode.CopyLoc z).
+    admit.
+  }
+  { guard_instruction (Bytecode.MoveLoc z).
+    admit.
+  }
+  { guard_instruction (Bytecode.StLoc z).
+    admit.
+  }
+  { guard_instruction (Bytecode.Call t).
+    admit.
+  }
+  { guard_instruction (Bytecode.CallGeneric t).
+    admit.
+  }
+  { guard_instruction (Bytecode.Pack t).
+    admit.
+  }
+  { guard_instruction (Bytecode.PackGeneric t).
+    admit.
+  }
+  { guard_instruction (Bytecode.Unpack t).
+    admit.
+  }
+  { guard_instruction (Bytecode.UnpackGeneric t).
+    admit.
+  }
+  { guard_instruction Bytecode.ReadRef.
+    admit.
+  }
+  { guard_instruction Bytecode.WriteRef.
+    admit.
+  }
+  { guard_instruction Bytecode.FreezeRef.
+    admit.
+  }
+  { guard_instruction (Bytecode.MutBorrowLoc z).
+    admit.
+  }
+  { guard_instruction (Bytecode.ImmBorrowLoc z).
     admit.
   }
 Admitted.
