CoqOfRust/move_sui/simulations/move_binary_format/file_format.v
@@ -501,7 +501,7 @@ pub enum SignatureToken {
 }
 *)
 Module SignatureToken.
-  Inductive t : Set := 
+  Inductive t : Set :=
   | Bool
   | U8
   | U64
